

# MATH 145B—HOMEWORK 6

Ricardo J. Acuña

(862079740)

1. (a) Reading from the picture:

$$C_1(S^1) = \{\lambda_0 e_0 + \lambda_1 e_1 + \lambda_2 e_2 \mid \lambda_i \in \mathbb{Z}\}$$

$$C_0(S^1) = \{\lambda_0 v_0 + \lambda_1 v_1 + \lambda_2 v_2 \mid \lambda_i \in \mathbb{Z}\}$$

$$C_n(S^1) = 0, \forall n \geq 2$$

$$\forall n \in \mathbb{N} : n \geq 2 \implies \mathbf{Ker} \partial_n = \mathbf{Im} \partial_n = 0$$

$$\implies \forall n \in \mathbb{N} : n \geq 2 : H_n(S^1) = \frac{0}{0} = 0$$

$$\partial_1(e_0) = v_2 - v_0$$

$$\partial_1(e_1) = v_1 - v_2$$

$$\partial_1(e_2) = v_0 - v_1$$

$$\implies \mathbf{Im} \partial_1 = \langle v_2 - v_0, v_1 - v_2, v_0 - v_1 \rangle$$

$$v_0 - v_1 = -(v_2 - v_0 + v_1 - v_2) \implies \text{one of the generators is redundant}$$

$$\implies \mathbf{Im} \partial_1 = \langle v_2 - v_0, v_1 - v_2 \rangle$$

$$\text{Solve } \partial_1(\lambda_0 e_0 + \lambda_1 e_1 + \lambda_2 e_2) = \lambda_0(v_2 - v_0) + \lambda_1(v_1 - v_2) + \lambda_2(v_0 - v_1) = 0$$

$$\implies \lambda_0(v_2 - v_0) + \lambda_1(v_1 - v_2) + \lambda_2(v_0 - v_1) = (\lambda_2 - \lambda_0)v_0 + (\lambda_1 - \lambda_2)v_1 + (\lambda_0 - \lambda_1)v_2 = 0$$

$$\implies \lambda_2 - \lambda_0 = 0 \text{ and } \lambda_1 - \lambda_2 = 0 \text{ and } \lambda_0 - \lambda_1 = 0 \implies \lambda_2 = \lambda_0 \text{ and } \lambda_1 = \lambda_2 \text{ and } \lambda_0 = \lambda_1$$

$$\implies \lambda_0 = \lambda_1 = \lambda_2 := \lambda$$

$$\implies \partial_1(\lambda(e_0 + e_1 + e_2)) = 0$$

$$\implies \mathbf{Ker} \partial_1 = \langle e_0 + e_1 + e_2 \rangle$$

$$\implies H_1(S^1) = \frac{\mathbf{Ker} \partial_1}{\mathbf{Im} \partial_1} = \frac{\langle e_0 + e_1 + e_2 \rangle}{0} = \mathbb{Z}$$

$$\partial_0(v_0) = \partial_0(v_1) = \partial_0(v_2) = 0$$

$$\implies \mathbf{Im} \partial_0 = 0 \text{ and } \mathbf{Ker} \partial_0 = \langle v_0, v_1, v_2 \rangle$$

$$\implies H_0(S^1) = \frac{\mathbf{Ker} \partial_0}{\mathbf{Im} \partial_1} = \frac{\langle v_0, v_1, v_2 \rangle}{\langle v_2 - v_0, v_1 - v_2 \rangle}$$

$$\text{One can change the basis of } C_0(S^1) = \mathbf{Ker} \partial_0 \text{ as such: } \langle v_0, v_1, v_2 \rangle = \langle v_0, v_1 - v_2, v_2 - v_0 \rangle$$

$$\implies H_0(S^1) = \frac{\langle v_0, v_1 - v_2, v_2 - v_0 \rangle}{\langle v_2 - v_0, v_1 - v_2 \rangle} = \langle v_0 \rangle = \mathbb{Z}$$

So,

$$H_n(Annulus) = \begin{cases} \mathbb{Z}, & n \in \{0, 1\} \\ 0, & \text{else} \end{cases}$$

**5. (a)**  $\forall n \in \mathbb{N} : n \geq 3 \implies C_n(S^2) = 0$

$$C_2(S^2) = \{\lambda f | \lambda \in \mathbb{Z}\}$$

$$C_1(S^2) = 0,$$

$$C_0(S^2) = \{\lambda v | \lambda \in \mathbb{Z}\}$$

$\forall n \in \mathbb{N} : n \geq 3 \implies \mathbf{Im} \partial_n = 0 = \mathbf{Ker} \partial_n$ . Because they're all 0.

$f$  is the only element of  $C_2(S^2) \implies \partial_2(f) = 0 \implies \mathbf{Im} \partial_2 = 0$  and  $\mathbf{Ker} \partial_2 = \langle f \rangle$

$$\implies H_2(S^2) = \frac{\mathbf{Ker} \partial_2}{\mathbf{Im} \partial_3} = \frac{\langle f \rangle}{0} = \langle f \rangle = \mathbb{Z}$$

0 is the only element of  $C_1(S^2) \implies \partial_1(0) = 0 \implies \mathbf{Im} \partial_1 = 0$  and  $\mathbf{Ker} \partial_1 = 0$

$v$  is the only element of  $C_0(S^2) \implies \partial_0(v) = 0 \implies \mathbf{Im} \partial_0 = 0$  and  $\mathbf{Ker} \partial_0 = \langle v \rangle$

$$\implies H_0(S^2) = \frac{\mathbf{Ker} \partial_0}{\mathbf{Im} \partial_1} = \frac{\langle v \rangle}{0} = \langle v \rangle = \mathbb{Z}$$

So,

$$H_n(S^2) = \begin{cases} \mathbb{Z}, & n \in \{0, 2\} \\ 0, & \text{else} \end{cases}$$

$$7. \textbf{(a)} \quad C_2(S^2) = \{\lambda f | \lambda \in \mathbb{Z}\}$$

$$C_1(\mathbb{R}P^2) = \{\lambda_0 a + \lambda_1 b | \lambda_i \in \mathbb{Z}\}$$

↓

$$C_0(\mathbb{R}P^2) = \{\lambda_0 v_0 + \lambda_1 v_1 | \lambda_i \in \mathbb{Z}\}$$

$$\forall n \in \mathbb{N} : n \geq 3 \implies C_n(\mathbb{R}P^2) = 0 \implies \mathbf{Im} \partial_n = 0 = \mathbf{Ker} \partial_n$$

$f$  is the only element of  $C_2(\mathbb{R}P^2) \implies \partial_2(f) = 2b - 2a$  since you twist each edge once.

$$\implies \mathbf{Im} \partial_2 = \langle 2(b - a) \rangle$$

$$x(b - a) = xb - xa = 0 \implies x = 0 \implies \mathbf{Ker} \partial_2 = 0$$

$$\implies H_n(\mathbb{R}P^2) = \frac{\mathbf{Ker} \partial_n}{\mathbf{Im} \partial_{n+1}} = \frac{0}{0} = 0, \text{ for } n \geq 2$$

$$\partial_1(a) = v - w \text{ and } \partial_1(b) = v - w$$

$$\implies \mathbf{Im} \partial_1 = \langle v - w \rangle$$

$$y_1(v - w) + y_2(v - w) = (y_1 + y_2)v - (y_1 + y_2)w = 0 \implies y_1 + y_2 = 0 \implies -y_1 = y_2$$

$$\implies \mathbf{Ker} \partial_1 = \langle b - a \rangle$$

$$\implies H_1(\mathbb{R}P^2) = \frac{\mathbf{Ker} \partial_1}{\mathbf{Im} \partial_2} = \frac{\langle b - a \rangle}{\langle 2(b - a) \rangle} = \frac{\mathbb{Z}}{2\mathbb{Z}} = \mathbb{Z}_2$$

$$\partial_0(v_0) = \partial_0(v_1) = 0 \implies \mathbf{Im} \partial_0 = 0 \text{ and } \mathbf{Ker} \partial_0 = \langle v_0, v_1 \rangle$$

One can change the generators  $\langle v_0, v_1 \rangle$  to  $\langle v_1 - v_0, v_0 \rangle$ .

$$\implies H_0(\mathbb{R}P^2) = \frac{\mathbf{Ker} \partial_0}{\mathbf{Im} \partial_1} = \frac{\langle v_0, v_1 \rangle}{\langle v_1 - v_0 \rangle} = \frac{\langle v_1 - v_0, v_0 \rangle}{\langle v_1 - v_0 \rangle} = \langle v_0 \rangle = \mathbb{Z}$$

So,

$$H_n(\mathbb{R}P^2) = \begin{cases} \mathbb{Z}, n = 0 \\ \mathbb{Z}_2, n = 1 \\ 0, \text{ else} \end{cases}$$

**10** Call the picture in the image  $K$

pf.

$$C_2(K) = \{\lambda_0 f_0 + \lambda_1 f_1 \mid \lambda_i \in \mathbb{Z}\}$$

$$C_1(K) = \{\lambda_0 b + \lambda_1 a \mid \lambda_i \in \mathbb{Z}\}$$

$$C_0(K) = \{\lambda_0 v \mid \lambda_i \in \mathbb{Z}\}$$

$$\partial_2(f_0) = a - b$$

$$\partial_2(f_1) = b$$

$$\implies \mathbf{Im} \partial_2 = \langle a - b, b \rangle = \langle a, b \rangle$$

$$x_1(a - b) + x_2 b = 0 \implies x_1 a + (x_2 - x_1)b = 0 \implies x_1 = 0, x_2 - x_1 = 0 \implies x_1 = x_2 = 0$$

$$\implies \mathbf{Ker} \partial_2 = 0$$

$$\mathbf{Im} \partial_3 = 0, \text{ since } C_3(K) = 0$$

$$\implies H_2(K) = \frac{0}{0} = 0$$

$$\mathbf{Ker} \partial_n = 0 \text{ and } \mathbf{Im} \partial_n = 0, \text{ for all } n \geq 3 \text{ since } C_n(K) = 0 \text{ then.}$$

$$\implies H_n(K) = \frac{0}{0} = 0, \text{ for all } n \geq 2$$

$$\partial_1(b) = 0$$

$$\partial_1(a) = 0$$

$$\implies \mathbf{Im} \partial_1 = 0$$

$$\implies \mathbf{Ker} \partial_1 = \langle a, b \rangle$$

$$\implies H_1(K) = \frac{\langle a, b \rangle}{\mathbf{Im} \partial_1} = \frac{\langle a, b \rangle}{\langle a, b \rangle} = 0$$

$$\partial_0(v) = 0$$

$$\implies \mathbf{Ker} \partial_0 = \langle v \rangle$$

$$H_0(K) = \frac{\langle v \rangle}{\mathbf{Im} \partial_1} = \frac{\langle v \rangle}{0} = \langle v \rangle = \mathbb{Z}$$

So,

$$H_n(K) = \begin{cases} \mathbb{Z}, & n = 0 \\ 0, & \text{else} \end{cases}$$

$$\text{For Torus } \chi(T^2) = \sum_{n=0}^{\infty} (-1)^n \dim C_n(K) = 1 - 2 + 1 + 0 + \dots = 0$$

$$\text{But, } \chi(K) = \sum_{n=0}^{\infty} (-1)^n \dim C_n(K) = 1 + 0 + 0 + \dots = 1$$

We didn't need to do any of this... You can get it from Euler's formula  $\chi = E - V + F$ .  $\chi_T = 0$ ,  $K$  has 1 more face so  $F' = F + 1 \implies \chi_K = 0 + 1 = 1$ .

The homology gets smaller, but the Euler characteristic gets bigger.

■

**12. (a)** See drawing of X.

$$C_2(X) = \{\lambda f \mid \lambda \in \mathbb{Z}\}$$

$$C_1(X) = \{\lambda_0 a + \lambda_1 b + \lambda_2 c + \lambda_3 d \mid \lambda_i \in \mathbb{Z}\}$$

$$C_0(X) = \{\lambda v \mid \lambda \in \mathbb{Z}\}$$

$$\partial_2(\lambda f) = 2\lambda(a + b + c)$$

$$\implies \mathbf{Im} \partial_2 = 2 \langle a + b + c \rangle$$

$$2\lambda(a + b + c) = 0 \implies \lambda = 0$$

$$\implies \mathbf{Ker} \partial_2 = 0$$

$$C_n(X) = 0, \text{ for } n \geq 3 \implies \mathbf{Im} \partial_n = 0$$

$$\implies H_n(X) = \frac{0}{0}, \text{ for } n \geq 2$$

$$\partial_1(a) = \partial_1(b) = \partial_1(c) = \partial_1(d) = 0$$

$$\implies \mathbf{Im} \partial_1 = 0$$

$$\implies \mathbf{Ker} \partial_1 = \langle a, b, c, d \rangle$$

$$\implies H_1(X) = \frac{\langle a, b, c, d \rangle}{2 \langle a + b + c \rangle} = \frac{\langle a + b + c, b, c, d \rangle}{2 \langle a + b + c \rangle} = \mathbb{Z} \oplus \mathbb{Z} \oplus \mathbb{Z} \oplus \mathbb{Z}_2$$

$$\partial_0(v) = 0$$

$$\implies \mathbf{Ker} \partial_0 = \langle v \rangle$$

$$\implies H_0(X) = \frac{\langle v \rangle}{0} = \mathbb{Z}$$

So

$$H_n(X) = \begin{cases} \mathbb{Z} & , n = 0 \\ \mathbb{Z} \oplus \mathbb{Z} \oplus \mathbb{Z} \oplus \mathbb{Z}_2 & , n = 1 \\ 0 & , \text{ else} \end{cases}$$